rhgfwpg

LeanGrow/F/EnvironmentManagement/SampleRegular/ExtractRec.lean
@@ -17,6 +17,14 @@ theorem test : n + 0 = n := by
 #check Nat.casesAuxOn
 #check_failure List.recAux
 
+#check isAuxRecursor
+#eval (do return isAuxRecursor (← getEnv) `Nat.recAux : CoreM _)
+#eval (do return isAuxRecursor (← getEnv) `Nat.rec : CoreM _)
+#eval (do return isAuxRecursor (← getEnv) `Nat.recOn : CoreM _)
+#eval (do return isRecCore (← getEnv) `Nat.recAux : CoreM _)
+#eval (do return isRecCore (← getEnv) `Nat.rec : CoreM _)
+
+
 
 def fac : Nat → Nat
 | 0 => 1
@@ -43,6 +51,7 @@ theorem test2 (n : Nat) : fac n ≥ 1 := by
 #check fac.eq_2
 
 #check_failure fac.match_1.eq_def
+#check_failure fac.match_1.eq_1
 
 def a := 42
 
@@ -58,7 +67,65 @@ theorem test3 : ∀ (n : ℕ), fac n ≥ 1 :=
       ) n
 
 
+def test4 (n : Nat) : Int := n
+
+#print test4
+
+#check congrArg
+
+#eval getEqnsFor? `fac
+#eval getEqnsFor? `a true
+#eval getUnfoldEqnFor? `fac
+#eval getUnfoldEqnFor? `a
+#eval getUnfoldEqnFor? `a true
+
+
+elab "redGoal" : tactic => do
+  let t ← Elab.Tactic.getMainTarget
+  let T ← whnf t
+  let τ ← reduce t false false false
+  logInfoAt (← getRef) s!"whnf: {(← ppExpr T)}\nreduced: {← ppExpr τ}"
+
+--#exit
+
+example : ∀ (n : ℕ), fac n ≥ 1 :=
+  fun n ↦ Nat.recAux
+    (le_refl 1)
+    (fun n ih ↦ by
+      have := le_trans ih (Nat.le_mul_of_pos_left (fac n) (Nat.succ_pos n))
+      redGoal
+      exact this
+      ) n
+
+def test5 := Nat.succ ((fun _ => 42) ())
+
+#print test5
+
+#check funext
+
+@[ext] -- also generates ex_iff !
+structure test6 where
+  a : Nat
+  b : Int
+
+#check test6.ext
+#print test6.ext
+-- but this isn't done by kernel, so shows up in samples ?
+
+#eval getEqnsFor? `test6 true
+#eval getUnfoldEqnFor? `test6 true
+
+#eval (do IO.println (Match.matchEqnsExt.getState (← getEnv) |>.eqns).toList : MetaM _)
+
+#check PHashSet.toList
+
+#check test6.mk
+
+
+example : test6.a (test6.mk 1 2) = 1 := rfl
+
 #exit
+
 
 def fib : Nat → Nat
 | 0 => 1
